Use order instead of relation in Wfrec, etc.

FOL/Cardinal.thy
@@ -66,58 +66,49 @@ definition Tup_image :: "i \<Rightarrow> i \<Rightarrow> i" where [rewrite]:
    of ordermap(r,y), where y < x under r.
 *)
 definition ordermap :: "i \<Rightarrow> i \<Rightarrow> i" where [rewrite]:
-  "ordermap(r,x) = wfrec(r, \<lambda>x f. Tup_image(f,rel_vsection(r,x)), x)"
+  "ordermap(r,x) = wfrec(r, \<lambda>x f. Tup_image(f,ord_pred(r,x)), x)"
 
 lemma ordermap_eq [rewrite]:
-  "wf(r) \<Longrightarrow> x \<in> source(r) \<Longrightarrow> ordermap(r,x) = {ordermap(r,y). y \<in> rel_vsection(r,x)}" by auto2
+  "wf(r) \<Longrightarrow> x \<in>. r \<Longrightarrow> ordermap(r,x) = {ordermap(r,y). y \<in> ord_pred(r,x)}" by auto2
 setup {* del_prfstep_thm @{thm ordermap_def} *}
 
 lemma ord_ordermap:
-  "wf(r) \<Longrightarrow> trans(r) \<Longrightarrow> x \<in> source(r) \<Longrightarrow> ord(ordermap(r,x))" by auto2
+  "wf(r) \<Longrightarrow> trans(r) \<Longrightarrow> x \<in>. r \<Longrightarrow> ord(ordermap(r,x))" by auto2
 setup {* add_forward_prfstep_cond @{thm ord_ordermap} [with_term "ordermap(?r,?x)"] *}
 
 (* The image of ordermap. *)
 definition ordertype :: "i \<Rightarrow> i" where [rewrite]:
-  "ordertype(r) = {ordermap(r,x). x \<in> source(r)}"
+  "ordertype(r) = {ordermap(r,x). x \<in>. r}"
 
 lemma ord_ordertype [forward]:
   "wf(r) \<Longrightarrow> trans(r) \<Longrightarrow> ord(ordertype(r))" by auto2
 
-definition linear_rel :: "i \<Rightarrow> o" where [rewrite]:
-  "linear_rel(r) \<longleftrightarrow> (\<forall>x\<in>source(r). \<forall>y\<in>source(r). rel(r,x,y) \<or> rel(r,y,x))"
-setup {* add_property_const @{term linear_rel} *}
-
-lemma linear_relD [forward]:
-  "linear_rel(r) \<Longrightarrow> x \<in> source(r) \<Longrightarrow> y \<in> source(r) \<Longrightarrow> \<not>rel(r,x,y) \<Longrightarrow> rel(r,y,x)" by auto2
-setup {* del_prfstep_thm_eqforward @{thm linear_rel_def} *}
-
 definition ordermap_fun :: "i \<Rightarrow> i" where [rewrite]:
-  "ordermap_fun(r) = Fun(source(r),ordertype(r), \<lambda>x. ordermap(r,x))"
+  "ordermap_fun(r) = Fun(carrier(r),ordertype(r), \<lambda>x. ordermap(r,x))"
 
 lemma ordermap_fun_type [typing]:
-  "ordermap_fun(r) \<in> source(r) \<rightarrow> ordertype(r)" by auto2
+  "ordermap_fun(r) \<in> carrier(r) \<rightarrow> ordertype(r)" by auto2
 
 lemma ordermap_fun_eval [rewrite]:
-  "x \<in> source(r) \<Longrightarrow> ordermap_fun(r)`x = ordermap(r,x)" by auto2
+  "x \<in> source(ordermap_fun(r)) \<Longrightarrow> ordermap_fun(r)`x = ordermap(r,x)" by auto2
 setup {* del_prfstep_thm @{thm ordermap_fun_def} *}
 
 lemma ordermap_inj [forward]:
-  "wf(r) \<Longrightarrow> trans(r) \<Longrightarrow> linear_rel(r) \<Longrightarrow> injective(ordermap_fun(r))"
+  "wf(r) \<Longrightarrow> trans(r) \<Longrightarrow> linorder(r) \<Longrightarrow> injective(ordermap_fun(r))"
 @proof
   @let "f = ordermap_fun(r)"
-  @let "A = source(r)"
-  @have "\<forall>x\<in>A. \<forall>y\<in>A. x \<noteq> y \<longrightarrow> f`x \<noteq> f`y" @with
-    @case "rel(r,x,y)" @with
+  @have "\<forall>x\<in>.r. \<forall>y\<in>.r. x \<noteq> y \<longrightarrow> f`x \<noteq> f`y" @with
+    @case "x \<le>\<^sub>r y" @with
       @have "ordermap(r,x) \<in> ordermap(r,y)"
     @end
-    @case "rel(r,y,x)" @with
+    @case "y \<le>\<^sub>r x" @with
       @have "ordermap(r,y) \<in> ordermap(r,x)"
     @end
   @end
 @qed
 
 lemma ordermap_bij [forward]:
-  "wf(r) \<Longrightarrow> trans(r) \<Longrightarrow> linear_rel(r) \<Longrightarrow> bijective(ordermap_fun(r))"
+  "wf(r) \<Longrightarrow> trans(r) \<Longrightarrow> linorder(r) \<Longrightarrow> bijective(ordermap_fun(r))"
   by auto2
 
 section \<open>Cardinals\<close>
@@ -131,7 +122,7 @@ definition card :: "i \<Rightarrow> o" where [rewrite]:
 section \<open>Basic properties of cardinals\<close>
 
 lemma cardinal_equipotent [resolve]:
-  "wf(r) \<Longrightarrow> trans(r) \<Longrightarrow> linear_rel(r) \<Longrightarrow> A = source(r) \<Longrightarrow> equipotent(A,cardinal(A))"
+  "wf(r) \<Longrightarrow> trans(r) \<Longrightarrow> linorder(r) \<Longrightarrow> A = carrier(r) \<Longrightarrow> equipotent(A,cardinal(A))"
 @proof
   @let "i = ordertype(r)"
   @have "equipotent(A,i)" @with
@@ -140,7 +131,7 @@ lemma cardinal_equipotent [resolve]:
 @qed
 
 lemma card_is_ordinal:
-  "wf(r) \<Longrightarrow> trans(r) \<Longrightarrow> linear_rel(r) \<Longrightarrow> A = source(r) \<Longrightarrow> ord(cardinal(A))"
+  "wf(r) \<Longrightarrow> trans(r) \<Longrightarrow> linorder(r) \<Longrightarrow> A = carrier(r) \<Longrightarrow> ord(cardinal(A))"
 @proof
   @let "i = ordertype(r)"
   @have "equipotent(A,i)" @with
