FOL/Wfrec.thy
@@ -2,79 +2,89 @@ theory Wfrec
 imports FixedPt
 begin
 
-definition rel_minimal :: "i \<Rightarrow> i \<Rightarrow> i \<Rightarrow> o" where [rewrite]:
-  "rel_minimal(r,Z,x) \<longleftrightarrow> (\<forall>y\<in>source(r). rel(r,y,x) \<longrightarrow> y \<notin> Z)"
+definition ord_minimal :: "i \<Rightarrow> i \<Rightarrow> i \<Rightarrow> o" where [rewrite]:
+  "ord_minimal(r,Z,x) \<longleftrightarrow> (\<forall>y\<in>.r. y \<le>\<^sub>r x \<longrightarrow> y \<notin> Z)"
 
 lemma rel_minimalD [forward]:
-  "y \<in> source(r) \<Longrightarrow> rel_minimal(r,Z,x) \<Longrightarrow> rel(r,y,x) \<Longrightarrow> y \<notin> Z" by auto2
-setup {* del_prfstep_thm_eqforward @{thm rel_minimal_def} *}
+  "y \<in>. r \<Longrightarrow> ord_minimal(r,Z,x) \<Longrightarrow> y \<le>\<^sub>r x \<Longrightarrow> y \<notin> Z" by auto2
+setup {* del_prfstep_thm_eqforward @{thm ord_minimal_def} *}
 
 definition wf :: "i \<Rightarrow> o" where [rewrite]:
-  "wf(r) \<longleftrightarrow> is_rel(r) \<and> (\<forall>Z\<in>Pow(source(r)). Z \<noteq> \<emptyset> \<longrightarrow> (\<exists>x\<in>Z. rel_minimal(r,Z,x)))"
+  "wf(r) \<longleftrightarrow> raworder(r) \<and> (\<forall>Z\<in>Pow(carrier(r)). Z \<noteq> \<emptyset> \<longrightarrow> (\<exists>x\<in>Z. ord_minimal(r,Z,x)))"
 setup {* add_property_const @{term wf} *}
 
-lemma wfD1 [forward]: "wf(r) \<Longrightarrow> is_rel(r)" by auto2
-lemma wfD2 [backward]: "wf(r) \<Longrightarrow> Z \<subseteq> source(r) \<Longrightarrow> Z \<noteq> \<emptyset> \<Longrightarrow> \<exists>x\<in>Z. rel_minimal(r,Z,x)" by auto2
+lemma wfD1 [forward]: "wf(r) \<Longrightarrow> raworder(r)" by auto2
+lemma wfD2 [backward]: "wf(r) \<Longrightarrow> Z \<noteq> \<emptyset> \<Longrightarrow> \<exists>x\<in>Z. ord_minimal(r,Z,x)" by auto2
 setup {* del_prfstep_thm_eqforward @{thm wf_def} *}
 
 (* Given \<langle>a,b\<rangle> \<in> r^+, take a' to be the predecessor of b in the chain from a to b. *)
 lemma rel_trans_cl_prev [backward]:
-  "is_rel(R) \<Longrightarrow> R' = rel_trans_cl(R) \<Longrightarrow> rel(R',a,b) \<Longrightarrow>
-   \<exists>a'\<in>source(R). rel(R,a',b) \<and> (a = a' \<or> rel(R',a,a'))"
+  "raworder(R) \<Longrightarrow> S = rel_trans_cl(R) \<Longrightarrow> a \<le>\<^sub>S b \<Longrightarrow>
+   \<exists>a'\<in>.R. a' \<le>\<^sub>R b \<and> (a = a' \<or> le(S,a,a'))"
 @proof
-  @induct "rel(rel_trans_cl(R),a,b)" "\<exists>a'\<in>source(R). rel(R,a',b) \<and> (a = a' \<or> rel(R',a,a'))"
+  @induct "le(rel_trans_cl(R),a,b)" "\<exists>a'\<in>.R. a' \<le>\<^sub>R b \<and> (a = a' \<or> a \<le>\<^sub>S a')"
 @qed
 
 lemma wf_trans_cl [forward]:
   "wf(r) \<Longrightarrow> wf(rel_trans_cl(r))"
 @proof
-  @let "A = source(r)"
+  @let "A = carrier(r)"
   @let "r' = rel_trans_cl(r)"
-  @have "\<forall>B\<in>Pow(A). B \<noteq> \<emptyset> \<longrightarrow> (\<exists>x\<in>B. rel_minimal(r',B,x))" @with
+  @have "\<forall>B\<in>Pow(A). B \<noteq> \<emptyset> \<longrightarrow> (\<exists>x\<in>B. ord_minimal(r',B,x))" @with
     @contradiction
-    @let "B' = {x\<in>A. \<exists>y\<in>B. rel(r',y,x)}"
-    @obtain "m\<in>B'" where "rel_minimal(r,B',m)"
+    @let "B' = {x\<in>A. \<exists>y\<in>B. le(r',y,x)}"
+    @obtain "m\<in>B'" where "ord_minimal(r,B',m)"
     @have "m \<in> B" @with
-      @obtain "y \<in> B" where "rel(r',y,m)"
-      @obtain "y' \<in> A" where "rel(r,y',m)" "(y=y' \<or> rel(r',y,y'))" @end
-    @have "\<forall>y\<in>source(r). rel(r',y,m) \<longrightarrow> y \<notin> B" @with
-      @obtain "y' \<in> A" where "rel(r,y',m)" "(y=y' \<or> rel(r',y,y'))" @end
+      @obtain "y \<in> B" where "le(r',y,m)"
+      @obtain "y' \<in> A" where "le(r,y',m)" "(y=y' \<or> le(r',y,y'))"
+    @end
+    @have "\<forall>y\<in>carrier(r). le(r',y,m) \<longrightarrow> y \<notin> B" @with
+      @obtain "y' \<in> A" where "le(r,y',m)" "(y=y' \<or> le(r',y,y'))"
+    @end
   @end
 @qed
 
 (* Well-founded induction *)
 lemma wf_induct [strong_induct]:
-  "wf(r) \<and> a \<in> source(r) \<Longrightarrow> \<forall>x\<in>source(r). (\<forall>y\<in>source(r). rel(r,y,x) \<longrightarrow> P(y)) \<longrightarrow> P(x) \<Longrightarrow> P(a)"
+  "wf(r) \<and> a \<in>. r \<Longrightarrow> \<forall>x\<in>.r. (\<forall>y\<in>.r. y \<le>\<^sub>r x \<longrightarrow> P(y)) \<longrightarrow> P(x) \<Longrightarrow> P(a)"
 @proof
-  @let "Z = {z \<in> source(r). \<not>P(z)}"
+  @let "Z = {z \<in>. r. \<not>P(z)}"
   @case "Z = \<emptyset>" @with @have "a \<notin> Z" @end
-  @obtain "m\<in>Z" where "rel_minimal(r,Z,m)"
+  @obtain "m\<in>Z" where "ord_minimal(r,Z,m)"
 @qed
 
-(* f is a family indexed by rel_vsection(r,a) (set of all x such that rel(r,x,a)),
+definition ord_pred :: "i \<Rightarrow> i \<Rightarrow> i" where [rewrite]:
+  "ord_pred(r,a) = {x\<in>.r. x \<le>\<^sub>r a}"
+setup {* register_wellform_data ("ord_pred(r,a)", ["a \<in>. r"]) *}
+
+lemma ord_predI [typing2,backward]: "raworder(r) \<Longrightarrow> x \<le>\<^sub>r a \<Longrightarrow> x \<in> ord_pred(r,a)" by auto2
+lemma ord_predE [forward]: "x \<in> ord_pred(r,a) \<Longrightarrow> x \<le>\<^sub>r a" by auto2
+setup {* del_prfstep_thm @{thm ord_pred_def} *}
+
+(* f is a family indexed by ord_pred(r,a) (set of all x such that le(r,x,a)),
    H is a meta-function from x and the segment of f before x to T. *)
 definition is_recfun :: "[i, i, [i, i] \<Rightarrow> i, i] \<Rightarrow> o" where [rewrite]:
-  "is_recfun(r,a,H,f) \<longleftrightarrow> f = Tup(rel_vsection(r,a), \<lambda>x. H(x, proj_set(f, rel_vsection(r,x))))"
+  "is_recfun(r,a,H,f) \<longleftrightarrow> f = Tup(ord_pred(r,a), \<lambda>x. H(x, proj_set(f, ord_pred(r,x))))"
 
 lemma is_recfun_is_family [forward]:
-  "is_recfun(r,a,H,f) \<Longrightarrow> is_family(f) \<and> source(f) = rel_vsection(r,a)" by auto2
+  "is_recfun(r,a,H,f) \<Longrightarrow> is_family(f) \<and> source(f) = ord_pred(r,a)" by auto2
 
 lemma is_recfun_eval [rewrite]:
-  "x \<in> source(f) \<Longrightarrow> is_recfun(r,a,H,f) \<Longrightarrow> f`x = H(x, proj_set(f, rel_vsection(r,x)))" by auto2
+  "x \<in> source(f) \<Longrightarrow> is_recfun(r,a,H,f) \<Longrightarrow> f`x = H(x, proj_set(f, ord_pred(r,x)))" by auto2
 
 lemma is_recfunI [backward2]:
-  "is_family(f) \<Longrightarrow> source(f) = rel_vsection(r,a) \<Longrightarrow>
-   \<forall>x\<in>source(f). f`x = H(x, proj_set(f, rel_vsection(r,x))) \<Longrightarrow> is_recfun(r,a,H,f)" by auto2
+  "is_family(f) \<Longrightarrow> source(f) = ord_pred(r,a) \<Longrightarrow>
+   \<forall>x\<in>source(f). f`x = H(x, proj_set(f, ord_pred(r,x))) \<Longrightarrow> is_recfun(r,a,H,f)" by auto2
 setup {* del_prfstep_thm @{thm is_recfun_def} *}
 
 (* Uniqueness of is_recfun: main result proved by well-founded induction,
    followed by two corollaries. *)
 lemma is_recfun_agree [forward]:
   "wf(r) \<Longrightarrow> trans(r) \<Longrightarrow> is_recfun(r,a,H,f) \<Longrightarrow> is_recfun(r,b,H,g) \<Longrightarrow>
-   \<forall>x. rel(r,x,a) \<longrightarrow> rel(r,x,b) \<longrightarrow> f`x = g`x"
+   \<forall>x. le(r,x,a) \<longrightarrow> le(r,x,b) \<longrightarrow> f`x = g`x"
 @proof
-  @have "\<forall>x. rel(r,x,a) \<longrightarrow> rel(r,x,b) \<longrightarrow> f`x = g`x" @with
-    @strong_induct "wf(r) \<and> x \<in> source(r)"
+  @have "\<forall>x. x \<le>\<^sub>r a \<longrightarrow> x \<le>\<^sub>r b \<longrightarrow> f`x = g`x" @with
+    @strong_induct "wf(r) \<and> x \<in>. r"
   @end
 @qed
 
@@ -83,7 +93,7 @@ lemma is_recfun_unique [forward]:
 
 lemma is_recfun_restrict_eq [forward]:
   "wf(r) \<Longrightarrow> trans(r) \<Longrightarrow> is_recfun(r,a,H,f) \<Longrightarrow> is_recfun(r,b,H,g) \<Longrightarrow>
-   rel(r,b,a) \<Longrightarrow> proj_set(f, rel_vsection(r,b)) = g" by auto2
+   b \<le>\<^sub>r a \<Longrightarrow> proj_set(f, ord_pred(r,b)) = g" by auto2
 setup {* del_prfstep_thm @{thm is_recfun_agree} *}
 
 (* Define recursive function using THE operator. *)
@@ -100,10 +110,10 @@ setup {* del_prfstep_thm @{thm the_recfun_def} *}
 
 (* Existence of recursive function, proved by a second well-founded induction. *)
 lemma unfold_the_recfun:
-  "wf(r) \<Longrightarrow> trans(r) \<Longrightarrow> a \<in> source(r) \<Longrightarrow> is_recfun(r,a,H,the_recfun(r,a,H))"
+  "wf(r) \<Longrightarrow> trans(r) \<Longrightarrow> a \<in>. r \<Longrightarrow> is_recfun(r,a,H,the_recfun(r,a,H))"
 @proof
-  @strong_induct "wf(r) \<and> a \<in> source(r)"
-  @let "f = Tup(rel_vsection(r,a), \<lambda>y. H(y, the_recfun(r,y,H)))"
+  @strong_induct "wf(r) \<and> a \<in>. r"
+  @let "f = Tup(ord_pred(r,a), \<lambda>y. H(y, the_recfun(r,y,H)))"
   @have "is_recfun(r,a,H,f)"
 @qed
 setup {* add_forward_prfstep_cond @{thm unfold_the_recfun} [with_term "the_recfun(?r,?a,?H)"] *}
@@ -114,23 +124,23 @@ definition wftrec :: "[i, [i, i] \<Rightarrow> i, i] \<Rightarrow> i" where [rew
 setup {* register_wellform_data ("wftrec(r,H,a)", ["a \<in> source(r)"]) *}
 
 lemma wftrec_unfold [rewrite]:
-  "wf(r) \<Longrightarrow> trans(r) \<Longrightarrow> a \<in> source(r) \<Longrightarrow>
-   wftrec(r,H,a) = H(a, Tup(rel_vsection(r,a), \<lambda>x. wftrec(r,H,x)))" by auto2
+  "wf(r) \<Longrightarrow> trans(r) \<Longrightarrow> a \<in>. r \<Longrightarrow>
+   wftrec(r,H,a) = H(a, Tup(ord_pred(r,a), \<lambda>x. wftrec(r,H,x)))" by auto2
 setup {* del_prfstep_thm @{thm wftrec_def} *}
 
 (* Definition that does not assume transitivity.
 
-   Assuming r is a well-founded relation and a is an element in source(r),
+   Assuming r is a well-founded order and a is an element in source(r),
    H is a meta-function indicating how to obtain value at x from a mapping
    from x and the family of values at the set r^-1(x).
 *)
 definition wfrec :: "[i, [i, i] \<Rightarrow> i, i] \<Rightarrow> i" where [rewrite]:
-  "wfrec(r,H,a) = wftrec(rel_trans_cl(r), \<lambda>x f. H(x, proj_set(f,rel_vsection(r,x))), a)"
+  "wfrec(r,H,a) = wftrec(rel_trans_cl(r), \<lambda>x f. H(x, proj_set(f,ord_pred(r,x))), a)"
 setup {* register_wellform_data ("wfrec(r,H,a)", ["a \<in> source(r)"]) *}
 
 lemma wfrec_unfold [rewrite]:
-  "wf(r) \<Longrightarrow> a \<in> source(r) \<Longrightarrow>
-   wfrec(r,H,a) = H(a, Tup(rel_vsection(r,a), \<lambda>x. wfrec(r,H,x)))" by auto2
+  "wf(r) \<Longrightarrow> a \<in>. r \<Longrightarrow>
+   wfrec(r,H,a) = H(a, Tup(ord_pred(r,a), \<lambda>x. wfrec(r,H,x)))" by auto2
 setup {* del_prfstep_thm @{thm wfrec_def} *}
 
 end
